Misc language clean up.

program_logic/ectx_language.v
@@ -3,7 +3,7 @@ From iris.program_logic Require Export language.
 
 (* We need to make thos arguments indices that we want canonical structure
    inference to use a keys. *)
-Class ectx_language (expr val ectx state : Type) := EctxLanguage {
+Class EctxLanguage (expr val ectx state : Type) := {
   of_val : val → expr;
   to_val : expr → option val;
   empty_ectx : ectx;
@@ -18,14 +18,14 @@ Class ectx_language (expr val ectx state : Type) := EctxLanguage {
 
   fill_empty e : fill empty_ectx e = e;
   fill_comp K1 K2 e : fill K1 (fill K2 e) = fill (comp_ectx K1 K2) e;
-  fill_inj K e1 e2 : fill K e1 = fill K e2 → e1 = e2;
+  fill_inj K :> Inj (=) (=) (fill K);
   fill_not_val K e : to_val e = None → to_val (fill K e) = None;
 
-  (* There are a whole lot of sensible axioms we could demand for comp_ectx
-     and empty_ectx. However, this one is enough. *)
+  (* There are a whole lot of sensible axioms (like associativity, and left and
+  right identity, we could demand for [comp_ectx] and [empty_ectx]. However,
+  positivity suffices. *)
   ectx_positive K1 K2 :
-    empty_ectx = comp_ectx K1 K2 →
-    K1 = empty_ectx ∧ K2 = empty_ectx;
+    comp_ectx K1 K2 = empty_ectx → K1 = empty_ectx ∧ K2 = empty_ectx;
 
   step_by_val K K' e1 e1' σ1 e2 σ2 ef :
     fill K e1 = fill K' e1' →
@@ -43,6 +43,7 @@ Class ectx_language (expr val ectx state : Type) := EctxLanguage {
     to_val e = None →
     K = empty_ectx;
 }.
+
 Arguments of_val {_ _ _ _ _} _.
 Arguments to_val {_ _ _ _ _} _.
 Arguments empty_ectx {_ _ _ _ _}.
@@ -56,7 +57,6 @@ Arguments of_to_val {_ _ _ _ _} _ _ _.
 Arguments val_stuck {_ _ _ _ _} _ _ _ _ _ _.
 Arguments fill_empty {_ _ _ _ _} _.
 Arguments fill_comp {_ _ _ _ _} _ _ _.
-Arguments fill_inj {_ _ _ _ _} _ _ _ _.
 Arguments fill_not_val {_ _ _ _ _} _ _ _.
 Arguments ectx_positive {_ _ _ _ _} _ _ _.
 Arguments step_by_val {_ _ _ _ _} _ _ _ _ _ _ _ _ _ _ _.
@@ -65,57 +65,57 @@ Arguments atomic_step {_ _ _ _ _} _ _ _ _ _ _ _.
 Arguments atomic_fill {_ _ _ _ _} _ _ _ _.
 
 (* From an ectx_language, we can construct a language. *)
-Section Language.
-  Context {expr val ectx state : Type} {Λ : ectx_language expr val ectx state}.
+Section ectx_language.
+  Context {expr val ectx state} {Λ : EctxLanguage expr val ectx state}.
   Implicit Types (e : expr) (K : ectx).
 
   Definition head_reducible (e : expr) (σ : state) :=
     ∃ e' σ' ef, head_step e σ e' σ' ef.
 
   Inductive prim_step (e1 : expr) (σ1 : state)
-    (e2 : expr) (σ2: state) (ef: option expr) : Prop :=
-  Ectx_step K e1' e2' :
-    e1 = fill K e1' → e2 = fill K e2' →
-    head_step e1' σ1 e2' σ2 ef → prim_step e1 σ1 e2 σ2 ef.
+      (e2 : expr) (σ2 : state) (ef : option expr) : Prop :=
+    Ectx_step K e1' e2' :
+      e1 = fill K e1' → e2 = fill K e2' →
+      head_step e1' σ1 e2' σ2 ef → prim_step e1 σ1 e2 σ2 ef.
 
   Lemma val_prim_stuck e1 σ1 e2 σ2 ef :
     prim_step e1 σ1 e2 σ2 ef → to_val e1 = None.
   Proof. intros [??? -> -> ?]; eauto using fill_not_val, val_stuck. Qed.
 
   Lemma atomic_prim_step e1 σ1 e2 σ2 ef :
-  atomic e1 → prim_step e1 σ1 e2 σ2 ef → is_Some (to_val e2).
+    atomic e1 → prim_step e1 σ1 e2 σ2 ef → is_Some (to_val e2).
   Proof.
     intros Hatomic [K e1' e2' -> -> Hstep].
     assert (K = empty_ectx) as -> by eauto 10 using atomic_fill, val_stuck.
-    eapply atomic_step; first done. by rewrite !fill_empty.
+    revert Hatomic; rewrite !fill_empty. eauto using atomic_step.
   Qed.
 
   Canonical Structure ectx_lang : language := {|
     language.expr := expr; language.val := val; language.state := state;
     language.of_val := of_val; language.to_val := to_val;
-    language.atomic := atomic; language.prim_step := prim_step;
+    language.atomic := atomic;
+    language.prim_step := prim_step;
     language.to_of_val := to_of_val; language.of_to_val := of_to_val;
-    language.val_stuck := val_prim_stuck; language.atomic_not_val := atomic_not_val;
+    language.val_stuck := val_prim_stuck;
+    language.atomic_not_val := atomic_not_val;
     language.atomic_step := atomic_prim_step
   |}.
 
   (* Some lemmas about this language *)
-  Lemma head_prim_reducible e σ :
-    head_reducible e σ → reducible e σ.
-  Proof.
-    intros (e'&?&?&?). do 3 eexists.
-    eapply Ectx_step with (K:=empty_ectx); rewrite ?fill_empty; done.
-  Qed.
+  Lemma head_prim_step e1 σ1 e2 σ2 ef :
+    head_step e1 σ1 e2 σ2 ef → prim_step e1 σ1 e2 σ2 ef.
+  Proof. apply Ectx_step with empty_ectx; by rewrite ?fill_empty. Qed.
+
+  Lemma head_prim_reducible e σ : head_reducible e σ → reducible e σ.
+  Proof. intros (e'&σ'&ef&?). eexists e', σ', ef. by apply head_prim_step. Qed.
 
   Lemma head_reducible_prim_step e1 σ1 e2 σ2 ef :
     head_reducible e1 σ1 → prim_step e1 σ1 e2 σ2 ef →
     head_step e1 σ1 e2 σ2 ef.
   Proof.
-    intros Hred Hstep. destruct Hstep as [? ? ? ? ? Hstep]; subst.
-    rename e1' into e1. rename e2' into e2.
-    destruct Hred as (e2'&σ2'&ef'&HstepK).
-    destruct (step_by_val K empty_ectx e1 (fill K e1) σ1 e2' σ2' ef')
-      as [K' [-> _]%ectx_positive];
+    intros (e2''&σ2''&ef''&?) [K e1' e2' -> -> Hstep].
+    destruct (step_by_val K empty_ectx e1' (fill K e1') σ1 e2'' σ2'' ef'')
+      as [K' [-> _]%symmetry%ectx_positive];
       eauto using fill_empty, fill_not_val, val_stuck.
     by rewrite !fill_empty.
   Qed.
@@ -129,16 +129,10 @@ Section Language.
       by exists (comp_ectx K K') e1' e2'; rewrite ?Heq1 ?Heq2 ?fill_comp.
     - intros e1 σ1 e2 σ2 ? Hnval [K'' e1'' e2'' Heq1 -> Hstep].
       destruct (step_by_val K K'' e1 e1'' σ1 e2'' σ2 ef) as [K' ->]; eauto.
-      rewrite -fill_comp in Heq1; apply fill_inj in Heq1.
+      rewrite -fill_comp in Heq1; apply (inj (fill _)) in Heq1.
       exists (fill K' e2''); rewrite -fill_comp; split; auto.
       econstructor; eauto.
   Qed.
-End Language.
-  
-Arguments ectx_lang {_ _ _ _} _ : clear implicits.
+End ectx_language.
 
-
-
-
-
-  
+Arguments ectx_lang {_ _ _ _} _.
