program_logic/ectx_weakestpre.v
@@ -1,14 +1,14 @@
-(** Some derived lemmas for ectx-based languages *)
 From iris.program_logic Require Export ectx_language weakestpre lifting.
 From iris.program_logic Require Import ownership.
 
 Section wp.
-Context {expr val ectx state: Type} {Λ : ectx_language expr val ectx state}
-        {Σ : iFunctor}.
+Context {expr val ectx state} {Λ : EctxLanguage expr val ectx state}.
+Context {Σ : iFunctor}.
 Implicit Types P : iProp (ectx_lang Λ) Σ.
 Implicit Types Φ : val → iProp (ectx_lang Λ) Σ.
 Implicit Types v : val.
 Implicit Types e : expr.
+Hint Resolve head_prim_reducible head_reducible_prim_step.
 
 Notation wp_fork ef := (default True ef (flip (wp ⊤) (λ _, True)))%I.
 
@@ -24,20 +24,14 @@ Lemma wp_lift_head_step E1 E2
   (|={E1,E2}=> ▷ ownP σ1 ★ ▷ ∀ e2 σ2 ef,
     (■ φ e2 σ2 ef ∧ ownP σ2) -★ |={E2,E1}=> WP e2 @ E1 {{ Φ }} ★ wp_fork ef)
   ⊢ WP e1 @ E1 {{ Φ }}.
-Proof.
-  intros. apply wp_lift_step;
-            eauto using head_prim_reducible, head_reducible_prim_step.
-Qed.
+Proof. eauto using wp_lift_step. Qed.
 
 Lemma wp_lift_pure_head_step E (φ : expr → option expr → Prop) Φ e1 :
   to_val e1 = None →
   (∀ σ1, head_reducible e1 σ1) →
   (∀ σ1 e2 σ2 ef, head_step e1 σ1 e2 σ2 ef → σ1 = σ2 ∧ φ e2 ef) →
   (▷ ∀ e2 ef, ■ φ e2 ef → WP e2 @ E {{ Φ }} ★ wp_fork ef) ⊢ WP e1 @ E {{ Φ }}.
-Proof.
-  intros. apply wp_lift_pure_step;
-            eauto using head_prim_reducible, head_reducible_prim_step.
-Qed.
+Proof. eauto using wp_lift_pure_step. Qed.
 
 Lemma wp_lift_atomic_head_step {E Φ} e1
     (φ : expr → state → option expr → Prop) σ1 :
@@ -47,10 +41,7 @@ Lemma wp_lift_atomic_head_step {E Φ} e1
     head_step e1 σ1 e2 σ2 ef → φ e2 σ2 ef) →
   (▷ ownP σ1 ★ ▷ ∀ v2 σ2 ef, ■ φ (of_val v2) σ2 ef ∧ ownP σ2 -★ Φ v2 ★ wp_fork ef)
   ⊢ WP e1 @ E {{ Φ }}.
-Proof.
-  intros. apply wp_lift_atomic_step;
-            eauto using head_prim_reducible, head_reducible_prim_step.
-Qed.
+Proof. eauto using wp_lift_atomic_step. Qed.
 
 Lemma wp_lift_atomic_det_head_step {E Φ e1} σ1 v2 σ2 ef :
   atomic e1 →
@@ -58,19 +49,12 @@ Lemma wp_lift_atomic_det_head_step {E Φ e1} σ1 v2 σ2 ef :
   (∀ e2' σ2' ef', head_step e1 σ1 e2' σ2' ef' →
     σ2 = σ2' ∧ to_val e2' = Some v2 ∧ ef = ef') →
   (▷ ownP σ1 ★ ▷ (ownP σ2 -★ Φ v2 ★ wp_fork ef)) ⊢ WP e1 @ E {{ Φ }}.
-Proof.
-  intros. apply wp_lift_atomic_det_step;
-            eauto using head_prim_reducible, head_reducible_prim_step.
-Qed.
+Proof. eauto using wp_lift_atomic_det_step. Qed.
 
 Lemma wp_lift_pure_det_head_step {E Φ} e1 e2 ef :
   to_val e1 = None →
   (∀ σ1, head_reducible e1 σ1) →
   (∀ σ1 e2' σ2 ef', head_step e1 σ1 e2' σ2 ef' → σ1 = σ2 ∧ e2 = e2' ∧ ef = ef')→
   ▷ (WP e2 @ E {{ Φ }} ★ wp_fork ef) ⊢ WP e1 @ E {{ Φ }}.
-Proof.
-  intros. apply wp_lift_pure_det_step;
-            eauto using head_prim_reducible, head_reducible_prim_step.
-Qed.
-
+Proof. eauto using wp_lift_pure_det_step. Qed.
 End wp.
